ok

SStructTT/SStruct/Runtime/Substitution.lean
@@ -2,13 +2,12 @@ import SStructTT.SStruct.Runtime.Resolution
 
 namespace SStruct.Erasure
 namespace Runtime
+open Dynamic
 variable {Srt : Type} [ord : SrtOrder Srt]
 
 @[aesop safe (rule_sets := [subst]) [constructors]]
 inductive AgreeSubst :
-  (Var -> Erasure.Tm Srt) ->
-  (Var -> Erasure.Tm Srt) ->
-  Nat -> Dynamic.Ctx Srt -> Heap Srt -> Prop
+  (Var -> Tm Srt) -> (Var -> Tm Srt) -> Nat -> Ctx Srt -> Heap Srt -> Prop
 where
   | nil {H σ σ'} :
     WR H ->
@@ -27,3 +26,117 @@ where
     H2 ;; m ▷ m' ->
     AgreeSubst σ σ' 0 Δ H1 ->
     AgreeSubst (m .: σ) (m' .: σ') 0 (A :⟨.ex, s⟩ Δ) H3
+
+lemma AgreeSubst.lower_image {Δ : Ctx Srt} {H σ σ' x s} :
+    AgreeSubst σ σ' x Δ H -> Lower Δ s -> HLower H s := by
+  intro agr lw; induction agr generalizing s
+  case nil hw =>
+    apply hw.trans
+    apply ord.e_min
+  case cons => cases lw <;> aesop
+  case wk_im => cases lw; aesop
+  case wk_ex wr hw2 mrg erm agr ih =>
+    cases lw; case ex le lw =>
+    have hw1 := ih lw
+    replace hw2 := hw2.trans le
+    apply mrg.lower_image hw1 hw2
+
+lemma AgreeSubst.subst_var {Δ : Ctx Srt} {H σ σ' i x} :
+    AgreeSubst σ σ' i Δ H -> x < i -> .var x = σ x := by
+  intro agr le; induction agr generalizing x
+  all_goals try trivial
+  case cons i _ _  agr ih =>
+    cases x with
+    | zero => asimp
+    | succ x =>
+      simp at le; asimp
+      have e := ih le
+      rw[<-e]; asimp
+
+lemma AgreeSubst.nf_subst {Δ : Ctx Srt} {H σ σ' i x m} :
+    AgreeSubst σ σ' i Δ H -> NF x m -> x ≤ i -> m = m.[σ] := by
+  intro agr nf lw; induction m generalizing Δ H σ σ' i x
+  all_goals simp_all
+  case var =>
+    asimp; apply agr.subst_var
+    apply nf.trans_le lw
+  case lam ih =>
+    asimp; apply ih
+    . apply AgreeSubst.cons agr
+      constructor; apply 0; constructor; apply ord.e
+    . assumption
+    . simp[lw]
+  case prj ihm ihn =>
+    have ⟨nf1, nf2⟩ := nf
+    asimp; split_ands
+    . aesop
+    . apply ihn
+      . apply AgreeSubst.cons
+        constructor; apply 0; constructor; apply ord.e
+        apply AgreeSubst.cons
+        constructor; apply 0; constructor; apply ord.e
+        apply agr
+      . aesop
+      . simp[lw]
+  all_goals asimp; try aesop
+
+lemma AgreeSubst.wr_heap {Δ : Ctx Srt} {H σ σ' i} :
+    AgreeSubst σ σ' i Δ H -> WR H := by
+  intro agr; induction agr
+  all_goals try aesop
+  case wk_ex wr2 _ mrg _ _ wr1 =>
+    apply mrg.merge_wr wr1 wr2
+
+def IdRename (i : Var) (ξ : Var -> Var) : Prop := ∀ x, x < i -> ξ x = x
+
+private lemma IdRename.zero : IdRename 0 (.+1) := by
+  intro x lw; cases lw
+
+private lemma IdRename.up {i ξ} :
+    IdRename i ξ -> IdRename (i + 1) (upren ξ) := by
+  intro idr x lt
+  cases x with
+  | zero => asimp
+  | succ x => simp at lt; asimp; apply idr _ lt
+
+omit ord in
+lemma NF.id_rename {m : Tm Srt} {i ξ} :
+    NF i m -> IdRename i ξ  -> m = m.[ren ξ] := by
+  intro nf idr; induction m generalizing i ξ
+  all_goals simp_all; try (solve| aesop)
+  case var => asimp; simp[idr _ nf]
+  case lam ih =>
+    asimp; rw[Tm.up_upren]; apply ih nf
+    apply idr.up
+  case app =>
+    have ⟨nf1, nf2⟩ := nf
+    asimp; aesop
+  case tup =>
+    have ⟨nf1, nf2⟩ := nf
+    asimp; aesop
+  case prj ih =>
+    have ⟨nf1, nf2⟩ := nf
+    asimp; split_ands
+    . aesop
+    . rw[show @upn (Tm Srt) _ _ 2 (ren ξ) = ren (upren (upren ξ)) by asimp]
+      apply ih nf2
+      apply idr.up.up
+  case ite =>
+    have ⟨nf1, nf2⟩ := nf
+    asimp; aesop
+  case rw => asimp; aesop
+
+lemma Resolve.id_rename {H : Heap Srt} {m m' i ξ} :
+    H ;; m ▷ m' -> WR H -> IdRename i ξ -> H ;; m.[ren ξ] ▷ m'.[ren ξ] := by
+  intro rs wr idr; induction rs generalizing i ξ
+  case var => sorry
+  case lam => sorry
+  case app => sorry
+  case tup => sorry
+  case prj => sorry
+  case tt => sorry
+  case ff => sorry
+  case ite => sorry
+  case rw => sorry
+  case ptr => sorry
+  case null => sorry
